Embedded STLC for CCCs and example program using presheafs

Haskell/Shim.hs
@@ -1,0 +1,13 @@
+import Test
+
+toInt :: Nat -> Int
+toInt O = 0
+toInt (S n) = 1 + toInt n
+
+fromInt :: Int -> Nat
+fromInt n | n < 0 = error "nat must be at least 0"
+fromInt 0 = O
+fromInt n = S (fromInt (n - 1))
+
+instance Show Nat where
+  show = show . toInt
