Language/CCCPL.v
@@ -1,0 +1,176 @@
+Set Universe Polymorphism.
+Set Asymmetric Patterns.
+
+(** Largely taken from CPDT
+  http://adam.chlipala.net/cpdt/html/ProgLang.html
+*)
+
+Require Import Spec.Category
+  Spec.CCC.CCC.
+Import Category.
+Import CCC. 
+
+Section STLC. 
+
+Context {U : Type} {ccat : CCat U}
+  {cmc : CMC U} `{CCCOps U (ccat := ccat)}.
+
+Require Import Coq.Lists.List.
+Import ListNotations.
+
+Local Open Scope obj.
+Local Open Scope morph.
+
+Fixpoint nprodT (xs : list U) : U := match xs with
+ | nil => unit
+ | x :: xs' => nprodT xs' * x
+ end.
+
+Inductive member {A} : A -> list A -> Type :=
+  | member_here : forall x xs, member x (x :: xs)
+  | memeber_there : forall x y ys, member x ys -> member x (y :: ys).
+
+Inductive termDB : list U -> U -> Type :=
+  | VarDB : forall G t, member t G -> termDB G t
+  | ConstDB : forall G (A : U), (nprodT G ~~> A) -> termDB G A
+  | AbsDB : forall G dom ran, termDB (dom :: G) ran -> termDB G (Func dom ran)
+  | AppDB : forall G dom ran, termDB G (Func dom ran) -> termDB G dom -> termDB G ran.
+
+  Arguments ConstDB {G} _ _.
+
+Definition compile_DB {Γ : list U} (A : U) 
+  (e : termDB Γ A) : nprodT Γ ~~> A.
+Proof.
+induction e.
+- induction m; simpl. apply snd.
+  apply (IHm ∘ fst). 
+- assumption.
+- apply abstract. simpl in IHe. apply IHe.
+- eapply compose. eapply eval.
+  eapply pair; eassumption.
+Defined.
+
+Section Var.
+  Context {var : U -> Type}.
+
+    Inductive term : U -> Type :=
+    | Var : forall {t}, var t -> term t
+    | Const : forall {A : U}, (unit ~~> A) -> term A
+    | Abs  : forall {dom ran}, (var dom -> term ran) -> term (Func dom ran)
+    | App  : forall {dom ran}, term (Func dom ran) -> term dom -> term ran.
+  End Var.
+
+  Arguments term : clear implicits.
+
+  Definition Term t := forall var, term var t.
+
+  Definition stupidT {A} : Term (A ==> A).
+  Proof. unfold Term. intros. apply Abs.
+  intros. apply Var. assumption.
+  Defined.
+
+Section wf.
+    Context {var1 var2 : U -> Type}.
+
+    Record varEntry := {
+      Ty : U;
+      First : var1 Ty;
+      Second : var2 Ty
+    }.
+
+ Inductive wf : list varEntry -> forall {t}, term var1 t -> term var2 t -> Type :=
+    | WfVar : forall G t x x', member {| Ty := t; First := x; Second := x' |} G
+      -> wf G (Var x) (Var x')
+    | WfConst : forall G A (e e' : unit ~~> A), e == e' ->  wf G (Const e) (Const e')
+    | WfAbs : forall G dom ran (e1 : _ dom -> term _ ran) e1',
+      (forall x1 x2, wf ({| First := x1; Second := x2 |} :: G) (e1 x1) (e1' x2))
+      -> wf G (Abs e1) (Abs e1')
+    | WfApp : forall G dom ran (e1 : term _ (Func dom ran)) (e2 : term _ dom) e1' e2',
+      wf G e1 e1'
+      -> wf G e2 e2'
+      -> wf G (App e1 e2) (App e1' e2').
+  End wf.
+
+  Definition Wf {t} (E : Term t) := forall var1 var2, wf nil (E var1) (E var2).
+
+  Lemma member_map {A B} (f : A -> B) {x : A} {xs : list A}
+   (elem : member x xs)
+  : member (f x) (List.map f xs).
+  Proof.
+  induction elem; simpl. constructor. constructor. assumption.
+  Defined.
+
+  Definition phoas_to_DB_helper {A}
+   (e1 : term (fun _ => True) A) (e2 : term (fun _ => True) A) Γ
+  (wellformed : wf Γ e1 e2)
+  : termDB (List.map Ty Γ) A.
+  Proof.
+  induction wellformed.
+  - apply VarDB. apply (member_map Ty) in m. apply m.
+  - apply ConstDB. exact (e ∘ tt).
+  - simpl in *. apply AbsDB. apply X; auto. 
+  - eapply AppDB; eauto.
+  Defined.
+
+  Definition phoas_to_DB {A} (E : Term A) (wellformed : Wf E) : termDB nil A.
+  Proof.
+  pose proof (phoas_to_DB_helper (E (fun _ => True)) (E (fun _ => True)) nil).
+  simpl in X. apply X. apply wellformed.
+  Defined.
+
+  Definition compile_phoas {A} (E : Term A) (wellformed : Wf E) 
+    : unit ~~> A :=
+    compile_DB _ (phoas_to_DB E wellformed).
+
+End STLC.
+
+Hint Constructors member : member_db.
+
+Ltac proveWF := red; 
+  intros; repeat match goal with
+  | [ |- wf _ _ _ ] => constructor; intros
+  | [ |- member _ _ ] => eauto with member_db
+  end; intuition.
+
+  Delimit Scope stlc_scope with stlc.
+
+  Notation "!" := Var : stlc_scope.
+  Notation "#" := Const : stlc_scope.
+  Infix "@" := App (left associativity, at level 50) : stlc_scope.
+  Notation "'λ' x .. y => t " := (Abs (fun x => .. (Abs (fun y => t)) .. ))
+        (x binder, y binder, at level 200, right associativity)
+        : stlc_scope.
+  Notation "[ e ]" := (fun _ => e) : stlc_scope.
+
+(*
+  Definition konst {A B} : Term (A ==> B ==> A) := 
+    [ λ (x : _ A) y => ! x ]%stlc.
+
+  Lemma konstWF : forall A B, Wf (@konst A B).
+  Proof. proveWF.
+  Defined.
+
+  Axiom M : U -> U.
+
+  Axiom undefined : forall A, A.
+
+  Definition Bind {A B} : unit ~~> (M A ==> (A ==> M B) ==> M B)
+    := undefined _.
+
+  Definition Ret {A} : unit ~~> (A ==> M A) := undefined _.
+
+  Axiom Bool Real : U.
+
+  Definition coinflip : unit ~~> M Bool := undefined _.
+  Definition normal : unit ~~> (Bool ==> M Real) := undefined _.
+
+  Definition pair {A B} : unit ~~> (A ==> B ==> A * B) := undefined _.
+
+  Definition testExp : Term (M (Bool * Real)) :=
+    [ #Bind @ #coinflip @ (λ x => #Bind @ (#normal @ !x) @
+      (λ y => #Ret @ (#pair @ !x @ !y) )) ]%stlc.
+
+  Definition testExpWF : Wf testExp.
+  Proof. proveWF. Defined.
+*)
+  
